

Advanced Algebra II HW1

Sean Eli

January 20, 2022

Problem 1. Show $p(x) = x^3 - 2x - 2$ is irreducible over \mathbb{Q} . Let θ be a root of this polynomial. Compute

$$(1 + \theta)(1 + \theta + \theta^2) \quad \text{and} \quad \frac{1 + \theta}{1 + \theta + \theta^2}$$

in $\mathbb{Q}(\theta)$, as \mathbb{Q} -linear combinations of $1, \theta$, and θ^2 .

Solution. Since 2 divides the non-leading coefficients of $p(x)$, but 4 does not divide the “1” coefficient, Eisenstein’s criterion shows that $p(x)$ is irreducible in $\mathbb{Q}[x]$. Let $\theta \in \mathbb{C}$ be a root of $p(x)$. Since $p(x)$ is irreducible and has degree 3, we know that

$$\mathbb{Q}(\theta) = \{a + b\theta + c\theta^2 : a, b, c, \in \mathbb{Q}\},$$

and in this field that $\theta^3 = 2\theta + 2$. Thus

$$(1 + \theta)(1 + \theta + \theta^2) = \theta^3 + 2\theta^2 + 2\theta + 1 = 2\theta^2 + 4\theta + 3.$$

Next, since $p(x)$ is irreducible of degree 3, it is relatively prime to all quadratic polynomials in $\mathbb{Q}[x]$. Thus, from the division algorithm, there exist polynomials $a(x), b(x) \in \mathbb{Q}[x]$ with $a(x)(1 + x + x^2) + b(x)p(x) = 1$. Using long division twice, we find

$$\begin{aligned} x^3 - 2x - 2 &= (x^2 + x + 1)(x - 1) - (2x + 1), \\ 4(x^2 + x + 1) &= -(2x + 1)(-2x - 1) + 3. \end{aligned}$$

Solving the second equation for 3 and eliminating a $2x + 1$ term using the first equation gives

$$3 = (2x + 1)p(x) + (-2x^2 + x + 5)(x^2 + x + 1).$$

Since $\mathbb{Q}(\theta) \cong \mathbb{Q}[x] / \langle p(x) \rangle$, the above equation shows that $(1 + \theta + \theta^2)^{-1} = \frac{1}{3}(-2\theta^2 + \theta + 5)$ in $\mathbb{Q}(\theta)$. Thus

$$\frac{1 + \theta}{1 + \theta + \theta^2} = \frac{(1 + \theta)(-2\theta^2 + \theta + 5)}{3} = \frac{-2\theta^3 - \theta^2 + 6\theta + 5}{3} = \frac{-\theta^2 + 2\theta + 1}{3}.$$

■

Problem 2. Let K/F be a field extension of degree n . Show that for any $\alpha \in K$, the “left multiplication by α ” map $m_\alpha : K \rightarrow K$ given by $x \mapsto \alpha \cdot x$ is an F -linear transformation. Deduce that K is isomorphic to a subfield of the ring $\text{Mat}_n(F)$ of $n \times n$ matrices over F .

Proof. Let $\alpha \in K$: additivity of m_α follows from the distributive law in K , and F -scalar multiplication follows from commutative multiplication in K and F . Thus $m_\alpha : K \rightarrow K$ is F -linear. By fixing a basis $B = \{b_1, \dots, b_n\}$ for K over F , we can represent each m_α as an $n \times n$ diagonal matrix $[m_\alpha]_B$ with entries in F . The function $\phi : K \rightarrow \text{Mat}_n(F)$ given by $\alpha \mapsto [m_\alpha]_B$ is a ring homomorphism (since by definition of m_a , we have $m_a \circ m_b = m_b \circ m_a = m_{ab}$ and $m_a + m_b = m_{a+b}$ for any $a, b \in K$.) Injectivity of ϕ follows since if m_a is the zero matrix, then $ab_1 + \dots + ab_n = 0$, and we have $a = 0$. ■

Problem 3. Show that $p(x) = x^4 + 3x + 3$ is irreducible over $\mathbb{Q}(\sqrt[3]{2})$.

Proof. Since 3 divides the non-leading coefficients of $p(x)$, but 9 does not divide the constant coefficient, Eisenstein’s criterion shows that $p(x)$ is irreducible in $\mathbb{Q}[x]$. Then if θ is a root of $p(x)$, $[\mathbb{Q}(\theta) : \mathbb{Q}] = 4$. Since the minimal polynomial of $\sqrt[3]{2}$ over \mathbb{Q} is $x^3 - 2$, it follows that $[\mathbb{Q}(\sqrt[3]{2}) : \mathbb{Q}] = 3$. Since $\mathbb{Q}(\sqrt[3]{2})$ and $\mathbb{Q}(\theta)$ are both subfields of $\mathbb{Q}(\theta, \sqrt[3]{2})$, by the tower law, both 3 and 4 divide $[\mathbb{Q}(\theta, \sqrt[3]{2}) : \mathbb{Q}]$. Therefore 12 divides $[\mathbb{Q}(\theta, \sqrt[3]{2}) : \mathbb{Q}]$, and since

$$[\mathbb{Q}(\theta, \sqrt[3]{2}) : \mathbb{Q}] = [\mathbb{Q}(\theta, \sqrt[3]{2}) : \mathbb{Q}(\sqrt[3]{2})] \cdot [\mathbb{Q}(\sqrt[3]{2}) : \mathbb{Q}] = [\mathbb{Q}(\theta, \sqrt[3]{2}) : \mathbb{Q}(\sqrt[3]{2})] \cdot 3,$$

it follows that 4 divides $[\mathbb{Q}(\theta, \sqrt[3]{2}) : \mathbb{Q}(\sqrt[3]{2})]$. However this is at most 4 since $p(x)$ is degree 4, therefore $[\mathbb{Q}(\theta, \sqrt[3]{2}) : \mathbb{Q}(\sqrt[3]{2})] = 4$. It follows that $p(x)$ is the minimal polynomial for θ over $\mathbb{Q}(\sqrt[3]{2})$, which is irreducible. ■

Problem 4. Let K/F be a field extension, and let $\alpha \in K$. Prove that if $[F(\alpha) : F]$ is odd, then $F(\alpha) = F(\alpha^2)$.

Proof. Notice $F \subset F(\alpha^2) \subset F(\alpha)$. By the tower law,

$$[F(\alpha) : F] = [F(\alpha) : F(\alpha^2)] \cdot [F(\alpha^2) : F],$$

therefore $[F(\alpha) : F(\alpha^2)]$ must be odd. Since $F(\alpha^2) \subset F(\alpha) = F(\alpha^2, \alpha)$, and α is a root of $f(x) = x^2 - (\alpha^2) \in F(\alpha^2)[x]$, we conclude $[F(\alpha) : F(\alpha^2)]$ is at most two. Since it is odd, it must be 1, therefore $F(\alpha) = F(\alpha^2)$. ■

Problem 5. Let K_1 and K_2 be finite extensions of a field F , contained in a field K . Prove that the F -algebra $K_1 \otimes_F K_2$ is a field iff $[K_1 K_2 : F] = [K_1 : F][K_2 : F]$.

Proof. We may write $K_1 = F(a_1, \dots, a_n)$ and let $K_2 = F(b_1, \dots, b_m)$ where $\{a_i\}$ and $\{b_j\}$ are vector space bases. Then the elements $\{a_i b_j : i = 1, \dots, n, j = 1, \dots, m\}$ span $K_1 K_2$.

The F -bilinear map $K_1 \times K_2 \rightarrow K_1 K_2$ given by $(x, y) \mapsto xy$ induces an F -linear map $\phi : K_1 \otimes_F K_2 \rightarrow K_1 K_2$, by the universal property of the tensor product of modules. The map ϕ is surjective, since $a_i \otimes b_j \mapsto a_i b_j$, and therefore the (linear span of the) spanning set $\{a_i b_j\}$ is in the image. Moreover, ϕ is a ring homomorphism, since for generic tensors $\sum_{i=1}^{\ell} x_i \otimes y_i$ and $\sum_{j=1}^k z_j \otimes w_j$,

$$\begin{aligned} \phi \left(\sum_{i=1}^{\ell} x_i \otimes y_i \cdot \sum_{j=1}^k z_j \otimes w_j \right) &= \phi \left(\sum_{i,j} x_i z_j \otimes y_i w_j \right) = \sum_{i,j} \phi(x_i z_j \otimes y_i w_j) \\ &= \sum_{i,j} x_i y_i z_j w_j \\ &= \sum_{i=1}^{\ell} x_i y_i \cdot \sum_{j=1}^k z_j w_j \\ &= \phi \left(\sum_{i=1}^{\ell} x_i \otimes y_i \right) \cdot \phi \left(\sum_{j=1}^k z_j \otimes w_j \right) \end{aligned}$$

Recall the dimension of $K_1 \otimes_F K_2$ over F is mn . Since ϕ is surjective, then $[K_1 K_2 : F] = mn$ iff ϕ is a linear isomorphism, i.e. injective. Since ϕ is a ring homomorphism, it follows that $[K_1 K_2 : F] = mn$ iff $K_1 \otimes_F K_2 \cong K_1 K_2$ as rings. This proves the claim since $\ker \phi \neq 0$ if and only if $K_1 \otimes_F K_2$ has a nontrivial ideal, and is not a field. ■